<?xml version="1.0"?>
<rdf:RDF xmlns="https://www.niso.org/standards-committees/ssos/ssos01.owl"
     xml:base="https://www.niso.org/standards-committees/ssos/ssos01.owl"
     xmlns:owl="http://www.w3.org/2002/07/owl#"
     xmlns:rdf="http://www.w3.org/1999/02/22-rdf-syntax-ns#"
     xmlns:xml="http://www.w3.org/XML/1998/namespace"
     xmlns:xsd="http://www.w3.org/2001/XMLSchema#"
     xmlns:rdfs="http://www.w3.org/2000/01/rdf-schema#"
     xmlns:skos="http://www.w3.org/2004/02/skos/core#">
    <owl:Ontology rdf:about="https://www.niso.org/standards-committees/ssos/ssos01.owl"/>
    


    <!-- 
    ///////////////////////////////////////////////////////////////////////////////////////
    //
    // Annotation properties
    //
    ///////////////////////////////////////////////////////////////////////////////////////
     -->

    


    <!-- http://www.w3.org/2000/01/rdf-schema#comment -->

    <owl:AnnotationProperty rdf:about="http://www.w3.org/2000/01/rdf-schema#comment"/>
    


    <!-- http://www.w3.org/2002/07/owl#retired -->

    <owl:AnnotationProperty rdf:about="http://www.w3.org/2002/07/owl#retired"/>
    


    <!-- http://www.w3.org/2004/02/skos/core#altLabel -->

    <owl:AnnotationProperty rdf:about="http://www.w3.org/2004/02/skos/core#altLabel"/>
    


    <!-- 
    ///////////////////////////////////////////////////////////////////////////////////////
    //
    // Datatypes
    //
    ///////////////////////////////////////////////////////////////////////////////////////
     -->

    


    <!-- http://www.w3.org/1999/02/22-rdf-syntax-ns#PlainLiteral -->

    <rdfs:Datatype rdf:about="http://www.w3.org/1999/02/22-rdf-syntax-ns#PlainLiteral"/>
    


    <!-- http://www.w3.org/2001/XMLSchema#date -->

    <rdfs:Datatype rdf:about="http://www.w3.org/2001/XMLSchema#date"/>
    


    <!-- http://www.w3.org/2001/XMLSchema#int -->

    <rdfs:Datatype rdf:about="http://www.w3.org/2001/XMLSchema#int"/>
    


    <!-- http://www.w3.org/2001/XMLSchema#integer -->

    <rdfs:Datatype rdf:about="http://www.w3.org/2001/XMLSchema#integer"/>
    


    <!-- http://www.w3.org/2001/XMLSchema#language -->

    <rdfs:Datatype rdf:about="http://www.w3.org/2001/XMLSchema#language"/>
    


    <!-- http://www.w3.org/2001/XMLSchema#string -->

    <rdfs:Datatype rdf:about="http://www.w3.org/2001/XMLSchema#string"/>
    


    <!-- 
    ///////////////////////////////////////////////////////////////////////////////////////
    //
    // Object Properties
    //
    ///////////////////////////////////////////////////////////////////////////////////////
     -->

    


    <!-- http://www.w3.org/2002/07/owl#topObjectProperty -->

    <owl:ObjectProperty rdf:about="http://www.w3.org/2002/07/owl#topObjectProperty"/>
    


    <!-- https://www.niso.org/standards-committees/ssos/ssos01.owl#availableSince -->

    <owl:ObjectProperty rdf:about="https://www.niso.org/standards-committees/ssos/ssos01.owl#availableSince">
        <rdfs:subPropertyOf rdf:resource="http://www.w3.org/2002/07/owl#topObjectProperty"/>
        <rdfs:comment>Date a particular standard instance was made available for use.</rdfs:comment>
    </owl:ObjectProperty>
    


    <!-- https://www.niso.org/standards-committees/ssos/ssos01.owl#continuousMaintenance -->

    <owl:ObjectProperty rdf:about="https://www.niso.org/standards-committees/ssos/ssos01.owl#continuousMaintenance">
        <rdfs:subPropertyOf rdf:resource="https://www.niso.org/standards-committees/ssos/ssos01.owl#hasMaintenanceType"/>
        <rdfs:comment>The consideration of recommended changes to any part of a standard according to a documented schedule for consideration and action by a consensus body. 
[Based on the definition in ANSI 2021, Essential Requirements, Section 4: Maintenance.]</rdfs:comment>
    </owl:ObjectProperty>
    


    <!-- https://www.niso.org/standards-committees/ssos/ssos01.owl#createNew -->

    <owl:ObjectProperty rdf:about="https://www.niso.org/standards-committees/ssos/ssos01.owl#createNew">
        <rdfs:subPropertyOf rdf:resource="http://www.w3.org/2002/07/owl#topObjectProperty"/>
        <rdfs:comment>A project that creates a new standard instance (that is, no previously active standard instance exists).</rdfs:comment>
    </owl:ObjectProperty>
    


    <!-- https://www.niso.org/standards-committees/ssos/ssos01.owl#hasLifeCycleState -->

    <owl:ObjectProperty rdf:about="https://www.niso.org/standards-committees/ssos/ssos01.owl#hasLifeCycleState">
        <rdfs:subPropertyOf rdf:resource="http://www.w3.org/2002/07/owl#topObjectProperty"/>
        <rdf:type rdf:resource="http://www.w3.org/2002/07/owl#TransitiveProperty"/>
        <rdfs:range rdf:resource="https://www.niso.org/standards-committees/ssos/ssos01.owl#Active_standard"/>
        <rdfs:range rdf:resource="https://www.niso.org/standards-committees/ssos/ssos01.owl#In-development"/>
        <rdfs:range rdf:resource="https://www.niso.org/standards-committees/ssos/ssos01.owl#Inactive_standard"/>
        <rdfs:comment>Life cycle state of a standard instance. (See terms, standard, instance, and life cycle, above.)</rdfs:comment>
    </owl:ObjectProperty>
    


    <!-- https://www.niso.org/standards-committees/ssos/ssos01.owl#hasMaintenanceType -->

    <owl:ObjectProperty rdf:about="https://www.niso.org/standards-committees/ssos/ssos01.owl#hasMaintenanceType">
        <rdfs:subPropertyOf rdf:resource="http://www.w3.org/2002/07/owl#topObjectProperty"/>
        <rdfs:comment>Status assigned during review(s) of an active standard.</rdfs:comment>
    </owl:ObjectProperty>
    


    <!-- https://www.niso.org/standards-committees/ssos/ssos01.owl#isAdoptionOf -->

    <owl:ObjectProperty rdf:about="https://www.niso.org/standards-committees/ssos/ssos01.owl#isAdoptionOf">
        <rdfs:comment>When a standards instance is adopted by a Standards Organization (A) from the body of standards of another Standards Organization (B).</rdfs:comment>
    </owl:ObjectProperty>
    


    <!-- https://www.niso.org/standards-committees/ssos/ssos01.owl#isCorrectedBy -->

    <owl:ObjectProperty rdf:about="https://www.niso.org/standards-committees/ssos/ssos01.owl#isCorrectedBy">
        <rdfs:comment>When a standard instance has one or more corrections, errata, corrigenda, etc.</rdfs:comment>
    </owl:ObjectProperty>
    


    <!-- https://www.niso.org/standards-committees/ssos/ssos01.owl#isExtendedBy -->

    <owl:ObjectProperty rdf:about="https://www.niso.org/standards-committees/ssos/ssos01.owl#isExtendedBy">
        <rdfs:comment>When a standard instance has one or more additions, such as supplements or addenda.</rdfs:comment>
    </owl:ObjectProperty>
    


    <!-- https://www.niso.org/standards-committees/ssos/ssos01.owl#isIdenticalAdoptionOf -->

    <owl:ObjectProperty rdf:about="https://www.niso.org/standards-committees/ssos/ssos01.owl#isIdenticalAdoptionOf">
        <rdfs:subPropertyOf rdf:resource="https://www.niso.org/standards-committees/ssos/ssos01.owl#isAdoptionOf"/>
        <rdfs:comment>When a standard instance is adopted by a Standards Organization without modification.</rdfs:comment>
    </owl:ObjectProperty>
    


    <!-- https://www.niso.org/standards-committees/ssos/ssos01.owl#isModifiedAdoptionOf -->

    <owl:ObjectProperty rdf:about="https://www.niso.org/standards-committees/ssos/ssos01.owl#isModifiedAdoptionOf">
        <rdfs:subPropertyOf rdf:resource="https://www.niso.org/standards-committees/ssos/ssos01.owl#isAdoptionOf"/>
        <rdfs:comment>When a standard instance is adopted by a Standards Organization with modification.</rdfs:comment>
    </owl:ObjectProperty>
    


    <!-- https://www.niso.org/standards-committees/ssos/ssos01.owl#isReaffirmedAs -->

    <owl:ObjectProperty rdf:about="https://www.niso.org/standards-committees/ssos/ssos01.owl#isReaffirmedAs">
        <rdfs:subPropertyOf rdf:resource="http://www.w3.org/2002/07/owl#topObjectProperty"/>
        <rdfs:comment>When an active standard instance is reaffirmed.
Note 1: If a decision is taken to reconfirm (or reaffirm) a standard, the Active State continues (without interruption).
Note 2: The dated designation of a reaffirmed standard generally includes an indication of reaffirmation, for example, in the form of and additional date, such as “R2021.”</rdfs:comment>
    </owl:ObjectProperty>
    


    <!-- https://www.niso.org/standards-committees/ssos/ssos01.owl#isRevisedTo -->

    <owl:ObjectProperty rdf:about="https://www.niso.org/standards-committees/ssos/ssos01.owl#isRevisedTo">
        <rdfs:subPropertyOf rdf:resource="http://www.w3.org/2002/07/owl#topObjectProperty"/>
        <rdfs:comment>When a standard instance is revised by a new standard instance.</rdfs:comment>
    </owl:ObjectProperty>
    


    <!-- https://www.niso.org/standards-committees/ssos/ssos01.owl#isTranslatedFrom -->

    <owl:ObjectProperty rdf:about="https://www.niso.org/standards-committees/ssos/ssos01.owl#isTranslatedFrom">
        <rdfs:subPropertyOf rdf:resource="http://www.w3.org/2002/07/owl#topObjectProperty"/>
        <rdfs:domain rdf:resource="https://www.niso.org/standards-committees/ssos/ssos01.owl#Dated_reference"/>
        <rdfs:range>
            <owl:Restriction>
                <owl:onProperty rdf:resource="https://www.niso.org/standards-committees/ssos/ssos01.owl#Language"/>
                <owl:allValuesFrom rdf:resource="http://www.w3.org/2001/XMLSchema#language"/>
            </owl:Restriction>
        </rdfs:range>
        <rdfs:comment>The standard instance or manifestation from which a translation has been made.</rdfs:comment>
    </owl:ObjectProperty>
    


    <!-- https://www.niso.org/standards-committees/ssos/ssos01.owl#periodicMaintenance -->

    <owl:ObjectProperty rdf:about="https://www.niso.org/standards-committees/ssos/ssos01.owl#periodicMaintenance">
        <rdfs:subPropertyOf rdf:resource="https://www.niso.org/standards-committees/ssos/ssos01.owl#hasMaintenanceType"/>
        <rdfs:comment>the review of the entire standard and action to revise or reaffirm it on a set schedule, generally not to exceed five years from the date of its approval. 
[Based on the definition in ANSI 2021, Essential Requirements, Section 4: Maintenance.]</rdfs:comment>
    </owl:ObjectProperty>
    


    <!-- https://www.niso.org/standards-committees/ssos/ssos01.owl#stabilizedMaintenance -->

    <owl:ObjectProperty rdf:about="https://www.niso.org/standards-committees/ssos/ssos01.owl#stabilizedMaintenance">
        <rdfs:subPropertyOf rdf:resource="https://www.niso.org/standards-committees/ssos/ssos01.owl#hasMaintenanceType"/>
        <rdfs:comment>Acknowledges a standard that has ongoing effectiveness and has reached technological maturity and is thus exempt from a continuous or periodic review schedule. In some standards organizations, a standard is put in stabilized maintenance if it supports the continued viability of existing products or the servicing of equipment that is expected to have a long working life. 
[Based on ISO/IEC JTC 1 Directives 2020.]</rdfs:comment>
    </owl:ObjectProperty>
    


    <!-- https://www.niso.org/standards-committees/ssos/ssos01.owl#supersedes -->

    <owl:ObjectProperty rdf:about="https://www.niso.org/standards-committees/ssos/ssos01.owl#supersedes">
        <rdfs:comment>A standard instance that has been replaced by a newer instance that covers at least the same scope.</rdfs:comment>
    </owl:ObjectProperty>
    


    <!-- https://www.niso.org/standards-committees/ssos/ssos01.owl#Partitioned/SeparatedFrom -->

    <owl:ObjectProperty rdf:about="https://www.niso.org/standards-committees/ssos/ssos01.owl#Partitioned/SeparatedFrom">
        <owl:inverseOf rdf:resource="https://www.niso.org/standards-committees/ssos/ssos01.owl#consolidates/combines"/>
        <rdfs:comment>When a new instance of a standard was a part of a previously available standard instance that covered a portion of the new instance’s scope.</rdfs:comment>
    </owl:ObjectProperty>
    


    <!-- https://www.niso.org/standards-committees/ssos/ssos01.owl#consolidates/combines -->

    <owl:ObjectProperty rdf:about="https://www.niso.org/standards-committees/ssos/ssos01.owl#consolidates/combines">
        <rdfs:subPropertyOf rdf:resource="http://www.w3.org/2002/07/owl#topObjectProperty"/>
        <rdfs:comment>When a new instance of a standard combines two or more previously available standard instances.</rdfs:comment>
    </owl:ObjectProperty>
    


    <!-- 
    ///////////////////////////////////////////////////////////////////////////////////////
    //
    // Data properties
    //
    ///////////////////////////////////////////////////////////////////////////////////////
     -->

    


    <!-- http://www.w3.org/2002/07/owl#topDataProperty -->

    <owl:DatatypeProperty rdf:about="http://www.w3.org/2002/07/owl#topDataProperty"/>
    


    <!-- https://www.niso.org/standards-committees/ssos/ssos01.owl#Approval_Year -->

    <owl:DatatypeProperty rdf:about="https://www.niso.org/standards-committees/ssos/ssos01.owl#Approval_Year">
        <rdfs:range rdf:resource="http://www.w3.org/2001/XMLSchema#int"/>
        <rdfs:comment>The year the standard instance was approved for use. 
Note: Not always the year of Release_Date, which can be after.</rdfs:comment>
    </owl:DatatypeProperty>
    


    <!-- https://www.niso.org/standards-committees/ssos/ssos01.owl#Classifications -->

    <owl:DatatypeProperty rdf:about="https://www.niso.org/standards-committees/ssos/ssos01.owl#Classifications">
        <rdfs:subPropertyOf rdf:resource="http://www.w3.org/2002/07/owl#topDataProperty"/>
        <rdfs:range rdf:resource="http://www.w3.org/2001/XMLSchema#string"/>
        <rdfs:comment>Subject area and/or key terms/codes associated with a standard instance or manifestation.
Note 1: Users are encouraged to provide additional explicit classifications.</rdfs:comment>
    </owl:DatatypeProperty>
    


    <!-- https://www.niso.org/standards-committees/ssos/ssos01.owl#DOI -->

    <owl:DatatypeProperty rdf:about="https://www.niso.org/standards-committees/ssos/ssos01.owl#DOI">
        <rdfs:subPropertyOf rdf:resource="https://www.niso.org/standards-committees/ssos/ssos01.owl#ID"/>
        <rdfs:range rdf:resource="http://www.w3.org/2001/XMLSchema#string"/>
        <rdfs:comment>A digital object identifier (DOI) is a persistent identifier or handle used to identify objects uniquely, standardized by the International Organization for Standardization (ISO).
(From Wikipedia.)</rdfs:comment>
        <skos:altLabel>Digital object identifier</skos:altLabel>
    </owl:DatatypeProperty>
    


    <!-- https://www.niso.org/standards-committees/ssos/ssos01.owl#Dated_designation -->

    <owl:DatatypeProperty rdf:about="https://www.niso.org/standards-committees/ssos/ssos01.owl#Dated_designation">
        <rdfs:subPropertyOf rdf:resource="http://www.w3.org/2002/07/owl#topDataProperty"/>
        <rdfs:range rdf:resource="http://www.w3.org/2001/XMLSchema#string"/>
        <rdfs:comment>Reference to a specific standard instance.</rdfs:comment>
    </owl:DatatypeProperty>
    


    <!-- https://www.niso.org/standards-committees/ssos/ssos01.owl#Format -->

    <owl:DatatypeProperty rdf:about="https://www.niso.org/standards-committees/ssos/ssos01.owl#Format">
        <rdfs:subPropertyOf rdf:resource="http://www.w3.org/2002/07/owl#topDataProperty"/>
        <rdfs:range rdf:resource="http://www.w3.org/2001/XMLSchema#string"/>
        <rdfs:comment>The format of the standard instance or manifestation (e.g., https://docs.w3cub.com/http/basics_of_http/mime_types/complete_list_of_mime_types).</rdfs:comment>
    </owl:DatatypeProperty>
    


    <!-- https://www.niso.org/standards-committees/ssos/ssos01.owl#Full_Title -->

    <owl:DatatypeProperty rdf:about="https://www.niso.org/standards-committees/ssos/ssos01.owl#Full_Title">
        <rdfs:subPropertyOf rdf:resource="http://www.w3.org/2002/07/owl#topDataProperty"/>
        <rdfs:range rdf:resource="http://www.w3.org/2001/XMLSchema#string"/>
        <rdfs:comment>Contains the full title of the standard. Normally, this contains all the introductory, main, and complementary titles and subtitles in a combined form, possibly with punctuation and spacing added between title components. The full title is a good interchange option, to communicate the title of a standard.
(From ANSI/NISO Z39.102-2017, NISO STS, version 1.0.)
Note 1: Titles in different languages are to be identified by ISO 639-2 language tags.</rdfs:comment>
    </owl:DatatypeProperty>
    


    <!-- https://www.niso.org/standards-committees/ssos/ssos01.owl#ICS_Codes -->

    <owl:DatatypeProperty rdf:about="https://www.niso.org/standards-committees/ssos/ssos01.owl#ICS_Codes">
        <rdfs:subPropertyOf rdf:resource="https://www.niso.org/standards-committees/ssos/ssos01.owl#Classifications"/>
        <rdfs:range rdf:resource="http://www.w3.org/2001/XMLSchema#string"/>
        <rdfs:comment>The ICS (International Classification for Standards) is intended to serve as a structure for catalogues of international, regional, and national standards and other normative documents, and as a basis for standing-order systems for international, regional and national standards. It may also be used for classifying standards and normative documents in databases, libraries, etc.
The ICS is a hierarchical classification which consists of three levels.
(From ISO ICS, 7th Edition, 2015.)</rdfs:comment>
    </owl:DatatypeProperty>
    


    <!-- https://www.niso.org/standards-committees/ssos/ssos01.owl#ID -->

    <owl:DatatypeProperty rdf:about="https://www.niso.org/standards-committees/ssos/ssos01.owl#ID">
        <rdfs:subPropertyOf rdf:resource="http://www.w3.org/2002/07/owl#topDataProperty"/>
        <rdfs:range rdf:resource="http://www.w3.org/2001/XMLSchema#string"/>
        <rdfs:comment>An ID (or set of IDs) associated with a standard instance or manifestation.
Note 1: Users are encouraged to provide additional or specific IDs.</rdfs:comment>
    </owl:DatatypeProperty>
    


    <!-- https://www.niso.org/standards-committees/ssos/ssos01.owl#ISBN -->

    <owl:DatatypeProperty rdf:about="https://www.niso.org/standards-committees/ssos/ssos01.owl#ISBN">
        <rdfs:subPropertyOf rdf:resource="https://www.niso.org/standards-committees/ssos/ssos01.owl#ID"/>
        <rdfs:domain rdf:resource="https://www.niso.org/standards-committees/ssos/ssos01.owl#Dated_reference"/>
        <rdfs:range rdf:resource="http://www.w3.org/2001/XMLSchema#integer"/>
        <rdfs:comment>The International Standard Book Number is a numeric commercial book identifier which is intended to be unique.
(From Wikipedia.)</rdfs:comment>
    </owl:DatatypeProperty>
    


    <!-- https://www.niso.org/standards-committees/ssos/ssos01.owl#Internal_ID -->

    <owl:DatatypeProperty rdf:about="https://www.niso.org/standards-committees/ssos/ssos01.owl#Internal_ID">
        <rdfs:subPropertyOf rdf:resource="https://www.niso.org/standards-committees/ssos/ssos01.owl#ID"/>
        <rdfs:range rdf:resource="http://www.w3.org/2001/XMLSchema#string"/>
        <rdfs:comment>An organization-specific internal identifier of a standards instance.</rdfs:comment>
    </owl:DatatypeProperty>
    


    <!-- https://www.niso.org/standards-committees/ssos/ssos01.owl#Keywords -->

    <owl:DatatypeProperty rdf:about="https://www.niso.org/standards-committees/ssos/ssos01.owl#Keywords">
        <rdfs:subPropertyOf rdf:resource="https://www.niso.org/standards-committees/ssos/ssos01.owl#Classifications"/>
        <rdfs:range rdf:resource="http://www.w3.org/2001/XMLSchema#string"/>
        <rdfs:comment>A keyword records one specific term, key phrase, abbreviation, taxonomic structure, or other expression that is found within the text of a standards instance, or implied (broader, narrower, etc.) from terms found within the instance.
(Derived from ANSI/NISO Z39.102-2017, NISO STS, version 1.0.)</rdfs:comment>
    </owl:DatatypeProperty>
    


    <!-- https://www.niso.org/standards-committees/ssos/ssos01.owl#Language -->

    <owl:DatatypeProperty rdf:about="https://www.niso.org/standards-committees/ssos/ssos01.owl#Language">
        <rdfs:subPropertyOf rdf:resource="http://www.w3.org/2002/07/owl#topDataProperty"/>
        <rdfs:domain rdf:resource="https://www.niso.org/standards-committees/ssos/ssos01.owl#Manifestation"/>
        <rdfs:range rdf:resource="http://www.w3.org/2001/XMLSchema#language"/>
        <rdfs:comment>Language in which a particular standard instance or manifestation is written.
Note 1: Reference ISO 639-2 language codes.</rdfs:comment>
    </owl:DatatypeProperty>
    


    <!-- https://www.niso.org/standards-committees/ssos/ssos01.owl#Product_code -->

    <owl:DatatypeProperty rdf:about="https://www.niso.org/standards-committees/ssos/ssos01.owl#Product_code">
        <rdfs:subPropertyOf rdf:resource="https://www.niso.org/standards-committees/ssos/ssos01.owl#ID"/>
        <rdfs:range rdf:resource="http://www.w3.org/2001/XMLSchema#string"/>
        <rdfs:comment>A publisher- (or originator-) specific product identifier of a standards instance.</rdfs:comment>
    </owl:DatatypeProperty>
    


    <!-- https://www.niso.org/standards-committees/ssos/ssos01.owl#Project_ID -->

    <owl:DatatypeProperty rdf:about="https://www.niso.org/standards-committees/ssos/ssos01.owl#Project_ID">
        <rdfs:subPropertyOf rdf:resource="https://www.niso.org/standards-committees/ssos/ssos01.owl#ID"/>
        <rdfs:range rdf:resource="http://www.w3.org/2001/XMLSchema#string"/>
        <rdfs:comment>An organization-specific project identifier of a standards instance used prior to being an active standard instance.</rdfs:comment>
    </owl:DatatypeProperty>
    


    <!-- https://www.niso.org/standards-committees/ssos/ssos01.owl#Projected_Release_Date -->

    <owl:DatatypeProperty rdf:about="https://www.niso.org/standards-committees/ssos/ssos01.owl#Projected_Release_Date">
        <rdfs:range rdf:resource="http://www.w3.org/2001/XMLSchema#string"/>
        <rdfs:comment>Date a particular standard instance will likely be made available for use.</rdfs:comment>
    </owl:DatatypeProperty>
    


    <!-- https://www.niso.org/standards-committees/ssos/ssos01.owl#Reaffirmed_Date -->

    <owl:DatatypeProperty rdf:about="https://www.niso.org/standards-committees/ssos/ssos01.owl#Reaffirmed_Date">
        <rdfs:subPropertyOf rdf:resource="http://www.w3.org/2002/07/owl#topDataProperty"/>
        <rdfs:domain rdf:resource="https://www.niso.org/standards-committees/ssos/ssos01.owl#Dated_reference"/>
        <rdfs:range rdf:resource="http://www.w3.org/2001/XMLSchema#string"/>
        <rdfs:comment>Date the standard instance was “reaffirmed” or “reconfirmed.”
Note 1: If a decision is taken to reconfirm (or reaffirm) a standard, the Active State continues (without interruption).
Note 2: The dated designation of a reaffirmed standard generally includes an indication of reaffirmation, for example, in the form of and additional date, such as “R2021.”</rdfs:comment>
    </owl:DatatypeProperty>
    


    <!-- https://www.niso.org/standards-committees/ssos/ssos01.owl#Release_Date -->

    <owl:DatatypeProperty rdf:about="https://www.niso.org/standards-committees/ssos/ssos01.owl#Release_Date">
        <rdfs:subPropertyOf rdf:resource="http://www.w3.org/2002/07/owl#topDataProperty"/>
        <rdfs:range rdf:resource="http://www.w3.org/2001/XMLSchema#string"/>
        <rdfs:comment>Date a particular standard instance was made available for use.</rdfs:comment>
    </owl:DatatypeProperty>
    


    <!-- https://www.niso.org/standards-committees/ssos/ssos01.owl#Source_language -->

    <owl:DatatypeProperty rdf:about="https://www.niso.org/standards-committees/ssos/ssos01.owl#Source_language">
        <rdfs:range rdf:resource="http://www.w3.org/2001/XMLSchema#language"/>
        <rdfs:comment>The language of the standard instance from which a translation has been made.
Note 1: Reference ISO 639-2 language codes.</rdfs:comment>
    </owl:DatatypeProperty>
    


    <!-- https://www.niso.org/standards-committees/ssos/ssos01.owl#Subject -->

    <owl:DatatypeProperty rdf:about="https://www.niso.org/standards-committees/ssos/ssos01.owl#Subject">
        <rdfs:subPropertyOf rdf:resource="https://www.niso.org/standards-committees/ssos/ssos01.owl#Classifications"/>
        <rdfs:range rdf:resource="http://www.w3.org/2001/XMLSchema#string"/>
        <rdfs:comment>Name of one overarching category, broad classification, topic, or theme used to describe a standards document, as a higher-level descriptor of its content.
(From ANSI/NISO Z39.102-2017, NISO STS, version 1.0.)</rdfs:comment>
    </owl:DatatypeProperty>
    


    <!-- https://www.niso.org/standards-committees/ssos/ssos01.owl#Undated_designation -->

    <owl:DatatypeProperty rdf:about="https://www.niso.org/standards-committees/ssos/ssos01.owl#Undated_designation">
        <rdfs:subPropertyOf rdf:resource="http://www.w3.org/2002/07/owl#topDataProperty"/>
        <rdfs:range rdf:resource="http://www.w3.org/2001/XMLSchema#string"/>
        <rdfs:comment>Reference to a standard without indicating the instance.
Note 1: In many cases, an undated reference indicates the active instance of a standard.</rdfs:comment>
    </owl:DatatypeProperty>
    


    <!-- 
    ///////////////////////////////////////////////////////////////////////////////////////
    //
    // Classes
    //
    ///////////////////////////////////////////////////////////////////////////////////////
     -->

    


    <!-- https://www.niso.org/standards-committees/ssos/ssos01.owl#Active_standard -->

    <owl:Class rdf:about="https://www.niso.org/standards-committees/ssos/ssos01.owl#Active_standard">
        <rdfs:subClassOf rdf:resource="https://www.niso.org/standards-committees/ssos/ssos01.owl#Life_cycle_states"/>
        <owl:disjointWith rdf:resource="https://www.niso.org/standards-committees/ssos/ssos01.owl#Manifestation"/>
        <owl:disjointWith rdf:resource="https://www.niso.org/standards-committees/ssos/ssos01.owl#Withdrawn_standard"/>
        <rdfs:comment>status assigned by a standardizing body to a standard at the time of publication which remains in effect until inactive (for example, superseded, withdrawn, deprecated, or retired). 
Note 1: The status “active” does not indicate the validity or non-validity of a standard.
(adapted from DIN 820-4:2014)
Note 2: Synonym: current standard</rdfs:comment>
        <skos:altLabel>Current standard</skos:altLabel>
    </owl:Class>
    


    <!-- https://www.niso.org/standards-committees/ssos/ssos01.owl#Canceled_project -->

    <owl:Class rdf:about="https://www.niso.org/standards-committees/ssos/ssos01.owl#Canceled_project">
        <rdfs:subClassOf rdf:resource="https://www.niso.org/standards-committees/ssos/ssos01.owl#In-development"/>
        <rdfs:comment>status assigned by a standardizing body to a project that was aborted before reaching the “active” status</rdfs:comment>
    </owl:Class>
    


    <!-- https://www.niso.org/standards-committees/ssos/ssos01.owl#Dated_reference -->

    <owl:Class rdf:about="https://www.niso.org/standards-committees/ssos/ssos01.owl#Dated_reference">
        <rdfs:subClassOf rdf:resource="https://www.niso.org/standards-committees/ssos/ssos01.owl#Standard_reference"/>
        <rdfs:comment>reference to a specific standard instance</rdfs:comment>
        <skos:altLabel>Dated designation</skos:altLabel>
        <skos:altLabel>Dated designator</skos:altLabel>
        <skos:altLabel>Dated standard reference</skos:altLabel>
    </owl:Class>
    


    <!-- https://www.niso.org/standards-committees/ssos/ssos01.owl#Deprecated_standard -->

    <owl:Class rdf:about="https://www.niso.org/standards-committees/ssos/ssos01.owl#Deprecated_standard">
        <rdfs:subClassOf rdf:resource="https://www.niso.org/standards-committees/ssos/ssos01.owl#Inactive_standard"/>
        <skos:altLabel>Canceled standard</skos:altLabel>
        <skos:altLabel>Standard that is declared as being no longer active by means of a formal withdrawal procedure that entails that this particular inactive standard is no longer fit for purpose.
Note 1: Formal withdrawal is a procedure used by some standards-setting institutions e.g., if there are grave safety concerns regarding the content.
Note 2: Synonym: canceled standard</skos:altLabel>
    </owl:Class>
    


    <!-- https://www.niso.org/standards-committees/ssos/ssos01.owl#Drafting -->

    <owl:Class rdf:about="https://www.niso.org/standards-committees/ssos/ssos01.owl#Drafting">
        <rdfs:subClassOf rdf:resource="https://www.niso.org/standards-committees/ssos/ssos01.owl#In-development"/>
        <rdfs:comment>status assigned by a standardizing body to a standard project for the period of time between the initial framework for a standard and the agreement of a consensus on the technical content of a draft within a standardization committee 
Note 1: The consensus draft is sometimes referred to as committee draft.</rdfs:comment>
    </owl:Class>
    


    <!-- https://www.niso.org/standards-committees/ssos/ssos01.owl#External_comment_and_review -->

    <owl:Class rdf:about="https://www.niso.org/standards-committees/ssos/ssos01.owl#External_comment_and_review">
        <rdfs:subClassOf rdf:resource="https://www.niso.org/standards-committees/ssos/ssos01.owl#In-development"/>
        <rdfs:comment>status assigned by a standardizing body to a standard project for the period of time between making a consensus draft available for comments outside the standardization committee and the end of the review and the resolution of comments received during that period
Note 1: A draft made available for public comment is sometimes referred to as draft standard.
Note 2: In some standardizing bodies, commenting outside the standardization committee can be limited to a peer review.</rdfs:comment>
    </owl:Class>
    


    <!-- https://www.niso.org/standards-committees/ssos/ssos01.owl#Final_approval -->

    <owl:Class rdf:about="https://www.niso.org/standards-committees/ssos/ssos01.owl#Final_approval">
        <rdfs:subClassOf rdf:resource="https://www.niso.org/standards-committees/ssos/ssos01.owl#In-development"/>
        <rdfs:comment>status assigned by a standardizing body to a standard project for the period of time following the final resolution of comments and approval of the final content by the standardizing body
Note 1: The final decision of approval of a standards body to publish a standard sometimes takes the form of a vote on a final draft</rdfs:comment>
        <skos:altLabel>Formal approval</skos:altLabel>
    </owl:Class>
    


    <!-- https://www.niso.org/standards-committees/ssos/ssos01.owl#In-development -->

    <owl:Class rdf:about="https://www.niso.org/standards-committees/ssos/ssos01.owl#In-development">
        <rdfs:subClassOf rdf:resource="https://www.niso.org/standards-committees/ssos/ssos01.owl#Life_cycle_states"/>
        <rdfs:comment>status assigned by a standardizing body to a standard project for the period of time between first expression of an idea and publication of the standard.</rdfs:comment>
    </owl:Class>
    


    <!-- https://www.niso.org/standards-committees/ssos/ssos01.owl#Inactive_standard -->

    <owl:Class rdf:about="https://www.niso.org/standards-committees/ssos/ssos01.owl#Inactive_standard">
        <rdfs:subClassOf rdf:resource="https://www.niso.org/standards-committees/ssos/ssos01.owl#Life_cycle_states"/>
        <owl:disjointWith rdf:resource="https://www.niso.org/standards-committees/ssos/ssos01.owl#Manifestation"/>
        <rdfs:comment>status that is assigned by a standardizing body to a standard no longer active.
Note 1: The status “inactive” does not refer to the validity or non-validity of a standard. The terms “valid” and “invalid” are only used and established by contractual parties, depending on the application.
(adapted from DIN 820-3:2014)
Synonym: historical standard</rdfs:comment>
        <skos:altLabel>historical standard</skos:altLabel>
    </owl:Class>
    


    <!-- https://www.niso.org/standards-committees/ssos/ssos01.owl#Informative_reference -->

    <owl:Class rdf:about="https://www.niso.org/standards-committees/ssos/ssos01.owl#Informative_reference">
        <rdfs:subClassOf rdf:resource="https://www.niso.org/standards-committees/ssos/ssos01.owl#Standard_reference"/>
        <rdfs:comment>a reference that may be useful for the implementation of the referencing standard.</rdfs:comment>
    </owl:Class>
    


    <!-- https://www.niso.org/standards-committees/ssos/ssos01.owl#Life_cycle_states -->

    <owl:Class rdf:about="https://www.niso.org/standards-committees/ssos/ssos01.owl#Life_cycle_states">
        <rdfs:comment>Status assigned by a standardizing body to a standards project for a sequence of events within the standards life cycle.</rdfs:comment>
    </owl:Class>
    


    <!-- https://www.niso.org/standards-committees/ssos/ssos01.owl#Maintenance -->

    <owl:Class rdf:about="https://www.niso.org/standards-committees/ssos/ssos01.owl#Maintenance">
        <rdfs:subClassOf rdf:resource="https://www.niso.org/standards-committees/ssos/ssos01.owl#Active_standard"/>
        <rdfs:comment>status assigned during review(s) of an active standard 
Note 1: This review can have three mutually exclusive results
•  If a decision is taken to reconfirm (or reaffirm) a standard, the Active State continues (without interruption)
•  If a decision is taken to revise a standard, the Active State ends when the superseding standard is approved or published
•  If a decision is taken to withdraw a standard, the Active State ends when the withdrawal formally occurs
Note 2: If a decision is taken to revise or reaffirm a standard, the new work would be in the top-level In Development state.
Note 3: Review can take the forms of continuous maintenance, periodic maintenance, or stabilized maintenance:
•  Continuous maintenance is the consideration of recommended changes to any part of a standard according to a documented schedule for consideration and action by a consensus body. [Based on the definition in ANSI 2021, Essential Requirements, Section 4: Maintenance.]
•  Periodic maintenance is the review of the entire standard and action to revise or reaffirm it on a set schedule, generally not to exceed five years from the date of its approval. [Based on the definition in ANSI 2021, Essential Requirements, Section 4: Maintenance.]
•  Stabilized maintenance acknowledges a standard that has ongoing effectiveness and has reached technological maturity, and is thus exempt from a continuous or periodic review schedule. In some standards organizations, a standard is put in stabilized maintenance if it supports the continued viability of existing products or the servicing of equipment that is expected to have a long working life. [Based on ISO/IEC JTC 1 Directives 2020.]</rdfs:comment>
    </owl:Class>
    


    <!-- https://www.niso.org/standards-committees/ssos/ssos01.owl#Manifestation -->

    <owl:Class rdf:about="https://www.niso.org/standards-committees/ssos/ssos01.owl#Manifestation">
        <rdfs:subClassOf rdf:resource="https://www.niso.org/standards-committees/ssos/ssos01.owl#Standard"/>
        <rdfs:comment>an expression of an instance that can be uniquely distinguished by one or more characteristics
Note 1: Examples of distinguishing characteristics can be, among others, different file formats or content languages for the same standard instance.</rdfs:comment>
    </owl:Class>
    


    <!-- https://www.niso.org/standards-committees/ssos/ssos01.owl#Normative_reference -->

    <owl:Class rdf:about="https://www.niso.org/standards-committees/ssos/ssos01.owl#Normative_reference">
        <rdfs:subClassOf rdf:resource="https://www.niso.org/standards-committees/ssos/ssos01.owl#Standard_reference"/>
        <rdfs:comment>reference deemed indispensable for the implementation of the referencing standard.
Note 1: a normative reference is used in place of quoting detailed provisions from the referenced standard or other material.</rdfs:comment>
    </owl:Class>
    


    <!-- https://www.niso.org/standards-committees/ssos/ssos01.owl#Pre-drafting -->

    <owl:Class rdf:about="https://www.niso.org/standards-committees/ssos/ssos01.owl#Pre-drafting">
        <rdfs:subClassOf rdf:resource="https://www.niso.org/standards-committees/ssos/ssos01.owl#In-development"/>
        <rdfs:comment>status assigned by a standardizing body to a standard project for the period of time between the acceptance of a proposal for a standard project until the development of an initial framework for a standard
Note 1: The initial framework for a standard could be a scope or a working draft.</rdfs:comment>
    </owl:Class>
    


    <!-- https://www.niso.org/standards-committees/ssos/ssos01.owl#Pre-proposal -->

    <owl:Class rdf:about="https://www.niso.org/standards-committees/ssos/ssos01.owl#Pre-proposal">
        <rdfs:subClassOf rdf:resource="https://www.niso.org/standards-committees/ssos/ssos01.owl#In-development"/>
        <rdfs:comment>status assigned by a standardizing body to a standard project for the period of time between first expression of an idea and formal standardization proposal</rdfs:comment>
    </owl:Class>
    


    <!-- https://www.niso.org/standards-committees/ssos/ssos01.owl#Production_and_publication -->

    <owl:Class rdf:about="https://www.niso.org/standards-committees/ssos/ssos01.owl#Production_and_publication">
        <rdfs:subClassOf rdf:resource="https://www.niso.org/standards-committees/ssos/ssos01.owl#In-development"/>
        <rdfs:comment>status assigned by a standardizing body to a standard project for the period of time between final approval of a standard until publication of the standard. This period includes the production process of a standard within the standardizing body and may include a translation period.
Note 1: The act of final approval or publication changes the top-level status of a standard from “in development” to “active.
Note 2: The specific date at which an active (standard) instance is made available for use is sometimes referred to as publication date or date of issuance.</rdfs:comment>
    </owl:Class>
    


    <!-- https://www.niso.org/standards-committees/ssos/ssos01.owl#Proposal -->

    <owl:Class rdf:about="https://www.niso.org/standards-committees/ssos/ssos01.owl#Proposal">
        <rdfs:subClassOf rdf:resource="https://www.niso.org/standards-committees/ssos/ssos01.owl#In-development"/>
        <rdfs:comment>status assigned by a standardizing body to a standard project for the period of time between distribution of a formal proposal for a standard project and the final decision on the formal proposal
Note 1: Common activities here are review and evaluation of the formal proposal. The result is either acceptance or rejection of the formal proposal.
Note 2: The formal proposal is sometimes referred to as “New Work Item Proposal” or “New standardization proposal”.</rdfs:comment>
    </owl:Class>
    


    <!-- https://www.niso.org/standards-committees/ssos/ssos01.owl#Reference -->

    <owl:Class rdf:about="https://www.niso.org/standards-committees/ssos/ssos01.owl#Reference">
        <rdfs:comment>citation to another standard, part of a standard, or other material.</rdfs:comment>
    </owl:Class>
    


    <!-- https://www.niso.org/standards-committees/ssos/ssos01.owl#Retired_standard -->

    <owl:Class rdf:about="https://www.niso.org/standards-committees/ssos/ssos01.owl#Retired_standard">
        <rdfs:subClassOf rdf:resource="https://www.niso.org/standards-committees/ssos/ssos01.owl#Inactive_standard"/>
        <rdfs:comment>Deprecated standard that is not available to the public.
Note 1: Synonyms: archived standard, deleted standard, and rescinded standard</rdfs:comment>
        <skos:altLabel>Archived standard</skos:altLabel>
        <skos:altLabel>Deleted standard</skos:altLabel>
        <skos:altLabel>Rescinded standard</skos:altLabel>
    </owl:Class>
    


    <!-- https://www.niso.org/standards-committees/ssos/ssos01.owl#Standard -->

    <owl:Class rdf:about="https://www.niso.org/standards-committees/ssos/ssos01.owl#Standard">
        <rdfs:comment>A documented instance of rules, guidelines, or characteristics for activities and/or their results, established by consensus and approved by a recognized body, aimed at the achievement of the optimum degree of order in a given context.
Note 1: All instances identified by the same standard’s designation are often referred to as a standards’ family.
Source: NISO SSOS WG adapting definitions of pre-existing standards</rdfs:comment>
    </owl:Class>
    


    <!-- https://www.niso.org/standards-committees/ssos/ssos01.owl#Standard_reference -->

    <owl:Class rdf:about="https://www.niso.org/standards-committees/ssos/ssos01.owl#Standard_reference">
        <rdfs:subClassOf rdf:resource="https://www.niso.org/standards-committees/ssos/ssos01.owl#Reference"/>
        <rdfs:comment>citation to another standard, part of a standard, or other material.</rdfs:comment>
    </owl:Class>
    


    <!-- https://www.niso.org/standards-committees/ssos/ssos01.owl#Standards_organization -->

    <owl:Class rdf:about="https://www.niso.org/standards-committees/ssos/ssos01.owl#Standards_organization">
        <rdfs:comment>An organization that produces documented instances of rules, guidelines, or characteristics for activities and/or their results, established by consensus and approved by a recognized body, aimed at the achievement of the optimum degree of order in a given context.
Note 1: Reference acronyms in https://en.wikipedia.org/wiki/List_of_technical_standard_organizations.</rdfs:comment>
    </owl:Class>
    


    <!-- https://www.niso.org/standards-committees/ssos/ssos01.owl#Superseded_standard -->

    <owl:Class rdf:about="https://www.niso.org/standards-committees/ssos/ssos01.owl#Superseded_standard">
        <rdfs:subClassOf rdf:resource="https://www.niso.org/standards-committees/ssos/ssos01.owl#Inactive_standard"/>
        <rdfs:comment>standard that was replaced by a newer instance of the standard which covers at least the same scope
(adapted from DIN 820-3:2014)</rdfs:comment>
    </owl:Class>
    


    <!-- https://www.niso.org/standards-committees/ssos/ssos01.owl#Superseding_standard -->

    <owl:Class rdf:about="https://www.niso.org/standards-committees/ssos/ssos01.owl#Superseding_standard">
        <rdfs:subClassOf rdf:resource="https://www.niso.org/standards-committees/ssos/ssos01.owl#Active_standard"/>
        <rdfs:comment>standard that by itself or together with other standards, replaces another standard and covers at least the same scope
(adapted from DIN 820-3:2014)</rdfs:comment>
    </owl:Class>
    


    <!-- https://www.niso.org/standards-committees/ssos/ssos01.owl#Undated_reference -->

    <owl:Class rdf:about="https://www.niso.org/standards-committees/ssos/ssos01.owl#Undated_reference">
        <rdfs:subClassOf rdf:resource="https://www.niso.org/standards-committees/ssos/ssos01.owl#Standard_reference"/>
        <rdfs:comment>reference to a standard without indicating the instance
Note 1: In many cases, an undated reference indicates the active instance of a standard</rdfs:comment>
        <skos:altLabel>Undated designation</skos:altLabel>
        <skos:altLabel>Undated designator</skos:altLabel>
        <skos:altLabel>Undated standard reference</skos:altLabel>
    </owl:Class>
    


    <!-- https://www.niso.org/standards-committees/ssos/ssos01.owl#Withdrawn_standard -->

    <owl:Class rdf:about="https://www.niso.org/standards-committees/ssos/ssos01.owl#Withdrawn_standard">
        <rdfs:subClassOf rdf:resource="https://www.niso.org/standards-committees/ssos/ssos01.owl#Inactive_standard"/>
        <rdfs:comment>standard that is declared as being no longer active and its status is set to “inactive”
Note 1: Withdrawal is either with replacement/supersession, with partial replacement/supersession or without replacement/supersession.
Note 2: A document which has been withdrawn may continue to be used e.g., if this has been contractually agreed and/or its continued use is permitted by law.
Note 3: Cf. “deprecated standard.”</rdfs:comment>
    </owl:Class>
    


    <!-- 
    ///////////////////////////////////////////////////////////////////////////////////////
    //
    // General axioms
    //
    ///////////////////////////////////////////////////////////////////////////////////////
     -->

    <rdf:Description>
        <rdf:type rdf:resource="http://www.w3.org/2002/07/owl#AllDisjointClasses"/>
        <owl:members rdf:parseType="Collection">
            <rdf:Description rdf:about="https://www.niso.org/standards-committees/ssos/ssos01.owl#Active_standard"/>
            <rdf:Description rdf:about="https://www.niso.org/standards-committees/ssos/ssos01.owl#In-development"/>
            <rdf:Description rdf:about="https://www.niso.org/standards-committees/ssos/ssos01.owl#Inactive_standard"/>
        </owl:members>
    </rdf:Description>
    <rdf:Description>
        <rdf:type rdf:resource="http://www.w3.org/2002/07/owl#AllDisjointClasses"/>
        <owl:members rdf:parseType="Collection">
            <rdf:Description rdf:about="https://www.niso.org/standards-committees/ssos/ssos01.owl#Deprecated_standard"/>
            <rdf:Description rdf:about="https://www.niso.org/standards-committees/ssos/ssos01.owl#Retired_standard"/>
            <rdf:Description rdf:about="https://www.niso.org/standards-committees/ssos/ssos01.owl#Superseded_standard"/>
            <rdf:Description rdf:about="https://www.niso.org/standards-committees/ssos/ssos01.owl#Withdrawn_standard"/>
        </owl:members>
    </rdf:Description>
    <rdf:Description>
        <rdf:type rdf:resource="http://www.w3.org/2002/07/owl#AllDisjointClasses"/>
        <owl:members rdf:parseType="Collection">
            <rdf:Description rdf:about="https://www.niso.org/standards-committees/ssos/ssos01.owl#Drafting"/>
            <rdf:Description rdf:about="https://www.niso.org/standards-committees/ssos/ssos01.owl#External_comment_and_review"/>
            <rdf:Description rdf:about="https://www.niso.org/standards-committees/ssos/ssos01.owl#Final_approval"/>
            <rdf:Description rdf:about="https://www.niso.org/standards-committees/ssos/ssos01.owl#Pre-drafting"/>
            <rdf:Description rdf:about="https://www.niso.org/standards-committees/ssos/ssos01.owl#Pre-proposal"/>
            <rdf:Description rdf:about="https://www.niso.org/standards-committees/ssos/ssos01.owl#Production_and_publication"/>
            <rdf:Description rdf:about="https://www.niso.org/standards-committees/ssos/ssos01.owl#Proposal"/>
        </owl:members>
    </rdf:Description>
</rdf:RDF>



<!-- Generated by the OWL API (version 4.5.9.2019-02-01T07:24:44Z) https://github.com/owlcs/owlapi -->

